MLIR/Examples/SemanticsTests.lean
@@ -3,6 +3,7 @@ import MLIR.AST
 import MLIR.Dialects.ArithSemantics
 import MLIR.Dialects.FuncSemantics
 import MLIR.Dialects.ControlFlowSemantics
+import MLIR.Dialects.ScfSemantics
 open MLIR.AST
 
 namespace SemanticsTests
@@ -31,28 +32,197 @@ def Test.run (t: Test): String :=
   | .ok ((r, env), assertLog) => assertLog
 
 def trueval := Test.mk (func_ + arith) "trueval.mlir" [mlir_region| {
-  %true = "constant" () {value = 1: i1}: () -> i1
+  %true = "arith.constant" () {value = 1: i1}: () -> i1
   "cf.assert" (%true) {msg="<FAILED>"}: (i1) -> ()
 
-  %z = "constant" () {value = 0: i32}: () -> i32
+  %z = "arith.constant" () {value = 0: i32}: () -> i32
   "func.return" (%z): (i32) -> ()
 }]
 
 def add := Test.mk (func_ + arith) "add.mlir" [mlir_region| {
-  %r1 = "constant" () {value = 17: i5}: () -> i5
-  %r2 = "constant" () {value = 25: i5}: () -> i5
-  %r = "addi" (%r1, %r2): (i5, i5) -> i5
-  %e = "constant" () {value = 10: i5}: () -> i5
-  %b = "cmpi" (%r, %e) {predicate = 0 /- eq -/}: (i5, i5) -> i1
+  %r1 = "arith.constant" () {value = 17: i5}: () -> i5
+  %r2 = "arith.constant" () {value = 25: i5}: () -> i5
+  %r = "arith.addi" (%r1, %r2): (i5, i5) -> i5
+  %e = "arith.constant" () {value = 10: i5}: () -> i5
+  %b = "arith.cmpi" (%r, %e) {predicate = 0 /- eq -/}: (i5, i5) -> i1
   "cf.assert" (%b) {msg="<FAILED>"}: (i1) -> ()
 
-  %z = "constant" () {value = 0: i32}: () -> i32
+  %z = "arith.constant" () {value = 0: i32}: () -> i32
   "func.return" (%z): (i32) -> ()
+}]
+
+def sub := Test.mk (func_ + arith) "sub.mlir" [mlir_region| {
+  %_1 = "arith.constant" () {value = 8374: i16}: () -> i16
+  %_2 = "arith.constant" () {value = 12404: i16}: () -> i16
+
+  %r1 = "arith.subi" (%_2, %_1): (i16, i16) -> i16
+  %e1 = "arith.constant" () {value = 4030: i16}: () -> i16
+  %b1 = "arith.cmpi" (%r1, %e1) {predicate = 0 /- eq -/}: (i16, i16) -> i1
+  "cf.assert" (%b1) {msg="<FAILED>"}: (i1) -> ()
+
+  %r2 = "arith.subi" (%r1, %_1): (i16, i16) -> i16
+  %e2 = "arith.constant" () {value = 61192: i16}: () -> i16
+  %b2 = "arith.cmpi" (%r1, %e1) {predicate = 0 /- eq -/}: (i16, i16) -> i1
+  "cf.assert" (%b2) {msg="<FAILED>"}: (i1) -> ()
+
+
+  %z = "arith.constant" () {value = 0: i32}: () -> i32
+  "func.return" (%z): (i32) -> ()
+}]
+
+def xor := Test.mk (func_ + arith) "xor.mlir" [mlir_region| {
+  %r1 = "arith.constant" () {value = 17: i8}: () -> i8
+  %r2 = "arith.constant" () {value = 25: i8}: () -> i8
+  %r = "arith.xori" (%r1, %r2): (i8, i8) -> i8
+  %e = "arith.constant" () {value = 8: i8}: () -> i8
+  %b = "arith.cmpi" (%r, %e) {predicate = 0 /- eq -/}: (i8, i8) -> i1
+  "cf.assert" (%b) {msg="<FAILED>"}: (i1) -> ()
+
+  %z = "arith.constant" () {value = 0: i32}: () -> i32
+  "func.return" (%z): (i32) -> ()
+}]
+
+def rw1 := Test.mk (func_ + arith) "rw1.mlir" [mlir_region| {
+  %_1 = "arith.constant"() {value = 84: i8}: () -> i8
+  %_2 = "arith.constant"() {value = 28: i8}: () -> i8
+
+  %r1 = "arith.xori"(%_1, %_2): (i8, i8) -> i8
+  %e1 = "arith.constant"() {value = 72: i8}: () -> i8
+  %b1 = "arith.cmpi" (%r1, %e1) {predicate = 0 /- eq -/}: (i8, i8) -> i1
+  "cf.assert" (%b1) {msg="<FAILED>"}: (i1) -> ()
+
+  %r2 = "arith.andi"(%_1, %_2): (i8, i8) -> i8
+  %e2 = "arith.constant"() {value = 20: i8}: () -> i8
+  %b2 = "arith.cmpi" (%r2, %e2) {predicate = 0 /- eq -/}: (i8, i8) -> i1
+  "cf.assert" (%b2) {msg="<FAILED>"}: (i1) -> ()
+
+  %r3 = "arith.ori"(%_1, %_2): (i8, i8) -> i8
+  %e3 = "arith.constant"() {value = 92: i8}: () -> i8
+  %b3 = "arith.cmpi" (%r3, %e3) {predicate = 0 /- eq -/}: (i8, i8) -> i1
+  "cf.assert" (%b3) {msg="<FAILED>"}: (i1) -> ()
+
+  %r4 = "arith.addi"(%r1, %r2): (i8, i8) -> i8
+  %b4 = "arith.cmpi" (%r4, %r3) {predicate = 0 /- eq -/}: (i8, i8) -> i1
+  "cf.assert" (%b4) {msg="<FAILED>"}: (i1) -> ()
+
+  %r5 = "arith.addi"(%_1, %_2): (i8, i8) -> i8
+  %e5 = "arith.constant"() {value = 112: i8}: () -> i8
+  %b5 = "arith.cmpi" (%r5, %e5) {predicate = 0 /- eq -/}: (i8, i8) -> i1
+  "cf.assert" (%b5) {msg="<FAILED>"}: (i1) -> ()
+
+  %r6 = "arith.addi"(%r2, %r3): (i8, i8) -> i8
+  %b6 = "arith.cmpi" (%r6, %e5) {predicate = 0 /- eq -/}: (i8, i8) -> i1
+  "cf.assert" (%b6) {msg="<FAILED>"}: (i1) -> ()
+
+  %z = "arith.constant" () {value = 0: i32}: () -> i32
+  "func.return" (%z): (i32) -> ()
+}]
+
+def if_true := Test.mk (func_ + scf + arith) "if_true.mlir" [mlir_region| {
+  %b = "arith.constant" () {value = 1: i1}: () -> i1
+  %y = "scf.if"(%b) ({
+    %x1 = "arith.constant"() {value = 3: i16}: () -> i16
+    "scf.yield"(%x1): (i16) -> ()
+  }, {
+    %x2 = "arith.constant"() {value = 4: i16}: () -> i16
+    "scf.yield"(%x2): (i16) -> ()
+  }): (i1) -> i16
+
+  %e = "arith.constant"() {value = 3: i16}: () -> i16
+  %b1 = "arith.cmpi" (%y, %e) {predicate = 0 /- eq -/}: (i16, i16) -> i1
+  "cf.assert"(%b1) {msg="<FAILED>"}: (i1) -> ()
+
+  %z = "arith.constant" () {value = 0: i32}: () -> i32
+  "func.return" (%z): (i32) -> ()
+}]
+
+def if_false := Test.mk (func_ + scf + arith) "if_false.mlir" [mlir_region| {
+  %b = "arith.constant" () {value = 0: i1}: () -> i1
+  %y = "scf.if"(%b) ({
+    %x1 = "arith.constant"() {value = 3: i16}: () -> i16
+    "scf.yield"(%x1): (i16) -> ()
+  }, {
+    %x2 = "arith.constant"() {value = 4: i16}: () -> i16
+    "scf.yield"(%x2): (i16) -> ()
+  }): (i1) -> i16
+
+  %e = "arith.constant"() {value = 4: i16}: () -> i16
+  %b1 = "arith.cmpi" (%y, %e) {predicate = 0 /- eq -/}: (i16, i16) -> i1
+  "cf.assert"(%b1) {msg="<FAILED>"}: (i1) -> ()
+
+  %z = "arith.constant" () {value = 0: i32}: () -> i32
+  "func.return" (%z): (i32) -> ()
+}]
+
+def if_select := Test.mk (func_ + scf + arith) "if_select.mlir" [mlir_region| {
+  %b = "arith.constant" () {value = 1: i1}: () -> i1
+  %x1 = "arith.constant"() {value = 12: i16}: () -> i16
+  %x2 = "arith.constant"() {value = 16: i16}: () -> i16
+
+  %y1 = "scf.if"(%b) ({
+    "scf.yield"(%x1): (i16) -> ()
+  }, {
+    "scf.yield"(%x2): (i16) -> ()
+  }): (i1) -> i16
+  %y2 = "arith.select"(%b, %x1, %x2): (i1, i16, i16) -> i16
+
+  %b1 = "arith.cmpi" (%y1, %y2) {predicate = 0 /- eq -/}: (i16, i16) -> i1
+  "cf.assert"(%b1) {msg="<FAILED>"}: (i1) -> ()
+
+  %z = "arith.constant" () {value = 0: i32}: () -> i32
+  "func.return" (%z): (i32) -> ()
+}]
+
+-- We only check the return value of the last instruction because we don't
+-- yet implement the folding behavior of the loop, and we have no side effects
+def for_trivial := Test.mk (func_ + scf + arith) "for_trivial.mlir" [mlir_region| {
+  %lower = "arith.constant"() {value =  8: i32}: () -> i32
+  %upper = "arith.constant"() {value = 18: i32}: () -> i32
+  %step  = "arith.constant"() {value =  1: i32}: () -> i32
+
+  %r = "scf.for"(%lower, %upper, %step) ({
+    "scf.yield"(%step): (i32) -> ()
+  }): (i32, i32, i32) -> ()
+
+  %e = "arith.constant"() {value = 1: i32}: () -> i32
+  %b = "arith.cmpi"(%e, %r) {predicate = 0 /- eq -/}: (i32, i32) -> i1
+  "cf.assert"(%b) {msg="<FAILED>"}: (i1) -> ()
+
+  %z = "arith.constant" () {value = 0: i32}: () -> i32
+  "func.return" (%z): (i32) -> ()
+}]
+
+def for_bound := Test.mk (func_ + scf + arith) "for_bound.mlir" [mlir_region| {
+  %lower = "arith.constant"() {value =  0: index}: () -> index
+  %upper = "arith.constant"() {value = 18: index}: () -> index
+  %step  = "arith.constant"() {value =  1: index}: () -> index
+
+  "scf.for"(%lower, %upper, %step) ({
+    ^bb(%i: index):
+      %b1 = "arith.cmpi"(%i, %lower) {predicate = 5 /- sge -/}: (index, index) -> i1
+      "cf.assert"(%b1) {msg="<FAILED>"}: (i1) -> ()
+
+      %b2 = "arith.cmpi"(%i, %upper) {predicate = 3 /- sle -/}: (index, index) -> i1
+      "cf.assert"(%b2) {msg="<FAILED>"}: (i1) -> ()
+
+      "scf.yield"(%step): (index) -> ()
+  }): (index, index, index) -> ()
+
+  %z = "arith.constant" () {value = 0: index}: () -> index
+  "func.return" (%z): (index) -> ()
 }]
 
 def allTests: Array Test := #[
   trueval,
-  add
+  add,
+  sub,
+  xor,
+  rw1,
+  if_true,
+  if_false,
+  if_select,
+--  for_trivial,
+  for_bound
 ]
 
 def runAllTests: IO Bool :=
